Working quicksort

assignment 2/quicksort.dfy
@@ -2,112 +2,122 @@
  * sort an array ascendingly
  */
 
-method {:verify true}Quicksort(a: array<int>, lo: int, hi: int)
-  modifies a // needed for arrays (since they are objects, not values such as sequences)
-  requires 0 <= lo <= hi <= a.Length; // lo can be equal to high if there are no elements placed in front of the pivot
-  ensures Sorted(a, lo, hi);
-  // Make sure that all the elements are lower than the element after this segment
-  //ensures hi == a.Length || forall j :: lo <= j < hi ==> a[j] < a[hi];
-  // Make sure that all the elements are higher or equal than the element before this segment
-  //ensures lo == 0 || forall j :: lo <= j < hi ==> a[j] >= a[lo]
-  ensures forall k | 0 <= k < lo :: a[k] ==old(a[k]);
-  ensures forall k | hi <= k < a.Length :: a[k] == old(a[k]);
-  //ensures lo == a.Length || BetweenLower(a, 0, lo);
-  //ensures BetweenHigher(a, hi, a.Length-1);
-  ensures hi == a.Length || a[hi] == old(a[hi]);
-  //(exists p : int :: p < hi && p >= lo && forall i | lo <= i < p :: a[i] < a[p] && forall j | p <= i < hi :: a[j] > a[p]);
-  // make sure parts not affected are the same
-  ensures multiset(a[..]) == multiset(old(a[..]))
-  decreases hi-lo;
+method Partition(a: array<int>, lo: int, hi: int) returns (pivot: int)
+  modifies a;
+  requires 0 <= lo < hi < a.Length;
+  requires 0 < lo ==> Partitioned(a, 0, lo - 1, lo, hi);
+  requires hi < a.Length - 1 ==> Partitioned(a, lo, hi, hi + 1, a.Length - 1);
+
+  ensures lo <= pivot <= hi;
+  ensures forall k | 0 <= k < lo || hi < k < a.Length :: a[k] == old(a[k]);
+  ensures multiset(a[..]) == multiset(old(a[..]));
+  ensures a[pivot] == old(a[hi]);
+  ensures forall k | lo <= k <= hi && k < pivot :: a[k] < old(a[hi]);
+  ensures forall k | lo <= k <= hi && k >= pivot :: a[k] >= old(a[hi]);
+
+  ensures 0 < lo ==> Partitioned(a, 0, lo - 1, lo, hi);
+  ensures hi < a.Length - 1 ==> Partitioned(a, lo, hi, hi + 1, a.Length - 1);
+  ensures lo < pivot ==> Partitioned(a, 0, pivot - 1, pivot, pivot);
+  ensures pivot < hi ==> Partitioned(a, 0, pivot, pivot + 1, hi);
 {
-    //assert(10<5);
+  var pVal := a[hi];
+  pivot := lo; // Will eventually contain the index of the pivot after partitioning.
+  var j := lo;
 
-    // EG lo == 5
-    // EG hi == 6,7 do nothing
-    //assert(lo == a.Length || BetweenLower(a, 0, lo));
-
-    // If there is less then two element to sort return
-    if(lo > hi - 2){
-        return;
-    }
-  
-  var p, u := lo, lo + 1; // marks the pivot and the unsorted part.
-
-    // Pivot set to the first element of the list
-  var pNr := a[p];
-
-
-  assert(forall k | 0 <= k < lo :: a[k] ==old(a[k]));
-
-  while u < hi
-    /*
-      lo           p                      u                          hi
-      LLLLLLLLLLLLLPHHHHHHHHHHHHHHHHHHHHHHUUUUUUUUUUUUUUUUUUUUUUUUUUU
-
-    */
-    invariant lo <= p < u <= hi
-    invariant pNr == a[p];
-    invariant multiset(a[..]) == multiset(old(a[..]))
-    invariant forall k :: lo <= k < p ==> a[k] < pNr;
-    invariant forall k :: p < k < u ==> a[k] >= pNr;
-    invariant forall k | 0 <= k < lo :: a[k] ==old(a[k]);
-    invariant forall k | hi <= k < a.Length :: a[k] == old(a[k]);
-    decreases hi-u;
+  while (j < hi) 
+    decreases hi - j;
+    invariant lo <= pivot <= j <= hi; // pivot index and j remain inside bounds
+    invariant forall k | 0 <= k < lo || hi < k < a.Length :: a[k] == old(a[k]);
+    invariant a[hi] == pVal; // pivot value remains at the end of the array
+    invariant forall k | lo <= k < pivot :: a[k] < pVal; // values before pivot are smaller
+    invariant forall k | pivot <= k < j :: pVal <= a[k]; // values after pivot greater or equal
+    invariant multiset(a[..]) == multiset(old(a[..])) // array always contains the same values
+    invariant 0 < lo ==> Partitioned(a, 0, lo - 1, lo, hi);
+    invariant hi < a.Length - 1 ==> Partitioned(a, lo, hi, hi + 1, a.Length - 1);
   {
-    if(a[u] < pNr){
-      // swap two element such that the element lower than p is now at position p+1;
-      swap(a, p+1, u);
-      // swap the pivot and the element after it.      
-      swap(a, p, p+1);
-      // increase p;
-      p:= p+1; 
+    if (a[j] < pVal) {
+      swap(a, pivot, j);
+      pivot := pivot + 1;
     }
-    u:= u+1;
+
+    j := j + 1;
   }
-  assert(forall k | 0 <= k < lo :: a[k] ==old(a[k]));
 
-  assert(forall j :: p < j < hi ==> a[j] >= a[p]);
-  assert(forall j :: lo <= j < p ==> a[j] < a[p]);
-  assert(BetweenLower(a, lo, p));
-  assert(BetweenHigher(a, p, hi-1));
-
-  Quicksort(a, lo, p);
-  assert(forall j :: p < j < hi ==> a[j] >= a[p]);
-  
-  assert(Sorted(a, lo, p));
-
-  assert(Sorted(a, lo ,p+1));
-  assert(BetweenLower(a, lo, p));
-  
-  assert(forall j :: p < j < hi ==> a[j] >= a[p]);
-  //assert(forall j :: lo <= j < p ==> a[j] < a[p]);
-  Quicksort(a, p+1, hi);
-  //assert(forall j :: lo <= j < p ==> a[j] < a[p]);
-
-
-  assert(Sorted(a, p+1, hi));
-  assert(Sorted(a, p, hi));
-  
-  assert(Sorted(a, lo, hi));
-  assert(forall k | hi <= k < a.Length :: a[k] == old(a[k]));
-
+  swap(a, pivot, hi);
 }
 
-//predicate Sorted?(a:seq<int>, lo: int, hi:int){
-  //forall i,j a[i] <= a[j]
-  //forall k .... a[k] < a[k+1];
-//}
+method {:verify true}Quicksort(a: array<int>, lo: int, hi: int)
+  modifies a // needed for arrays (since they are objects, not values such as sequences)
+  requires 0 <= lo <= hi < a.Length;
+  requires 0 < lo ==> Partitioned(a, 0, lo - 1, lo, hi);
+  requires hi < a.Length - 1 ==> Partitioned(a, lo, hi, hi + 1, a.Length - 1);
+  ensures forall k | 0 <= k < lo || hi < k < a.Length :: a[k] == old(a[k]);
+  ensures Sorted(old(a), 0, lo) ==> Sorted(a, 0, lo);
+  ensures Sorted(old(a), hi, a.Length - 1) ==> Sorted(a, hi, a.Length - 1);
+  ensures Sorted(a, lo, hi);
+  ensures multiset(a[..]) == multiset(old(a[..]));
+  ensures 0 < lo ==> Partitioned(a, 0, lo - 1, lo, hi);
+  ensures hi < a.Length - 1 ==> Partitioned(a, lo, hi, hi + 1, a.Length - 1);
+  decreases hi-lo;
+{
+  if (lo == hi) {
+    return;
+  }
+
+  var pivot := Partition(a, lo, hi);
+  var loVal := a[lo];
+
+  if (pivot > lo) {
+    Quicksort(a, lo, pivot - 1);
+  } 
+
+  if (pivot < hi) {
+    Quicksort(a, pivot + 1, hi);
+  } 
+}
+
+/*----- Lemmas -----*/
+lemma {:induction false} test(a: array<int>, lo: int, hi: int, n: int)
+  requires 0 <= lo <= hi < a.Length;
+  requires Sorted(a, lo, hi);
+  requires n <= a[lo];
+  ensures forall k | lo <= k <= hi < a.Length :: n <= a[k];
+  decreases hi - lo;
+  {
+    if (lo == hi) {
+
+    } else {
+      test(a, lo + 1, hi, n);
+    }
+  }
+
+lemma {:induction false} lemmaSortedTransitive(a: array<int>, lo: int, hi: int)
+  // reads a;
+  requires 0 <= lo <= hi < a.Length;
+  requires Sorted(a, lo, hi);
+  ensures forall i,j | lo <= i <= j <= hi < a.Length :: a[i] <= a[j];
+  decreases hi - lo;
+  {
+    if (lo == hi) {
+
+    } else {
+      lemmaSortedTransitive(a, lo + 1, hi);
+      assert (a[lo] <= a[lo + 1]);
+    }
+  }
+
+predicate Partitioned(a: array<int>, lo1: int, hi1: int, lo2: int, hi2: int)
+  reads a;
+  requires 0 <= lo1 <= hi1 <= lo2 <= hi2 < a.Length;
+  {
+    forall i,j | lo1 <= i <= hi1 < lo2 <= j <= hi2 :: a[i] <= a[j]
+  }
 
 predicate Sorted(a:array<int>, lo: int, hi:int)
   reads a;
-  requires 0 <= lo <= hi <= a.Length;
-  //ensures (lo == a.Length || forall k | 0 <= k < lo :: a[k] < a[lo]);
-  ensures forall j | hi > j > a.Length :: a[j] < a[hi];
-  
+  requires 0 <= lo <= hi < a.Length;
   {
-    forall i :: lo < i < hi-1 ==> a[i] <= a[i+1]
-    //forall i, j :: lo < i < j < hi-1  ==> a[i] <= a[j]
-    //(forall i :: lo <= i < hi-1 ==> a[i] <= a[i+1]) || (forall i :: lo < i <= hi-1 ==> a[i-1] <= a[i])
+    forall i | lo <= i < hi :: a[i] <= a[i+1]
   }
 
 //All values before a certain index must be lower than this specific number
